Rough security arguments defined for PPRF and setup of implimentatino of PRS

puncturableprf.ec
@@ -12,7 +12,7 @@ type PK = {key : K; x : D option}.
 op dK: { K distr | is_lossless dK } as dK_ll.
 op F : K -> D -> R.
 
-module PuncturablePsuedoRF = {
+module PPRF1 = {
 
   (* Gets a key from distribution dK and create pK with no punture point *)
   proc init() : PK = {
@@ -44,10 +44,10 @@ module PuncturablePrfCorrectnessGame = {
     var k;
     var pk;
     var x1, x2;
-    k <@ PuncturablePsuedoRF.init();
-    pk <@ PuncturablePsuedoRF.puncture(xp, k);
-    x1 <@ PuncturablePsuedoRF.f(xi, k);
-    x2 <@ PuncturablePsuedoRF.f(xi, pk);
+    k <@ PPRF1.init();
+    pk <@ PPRF1.puncture(xp, k);
+    x1 <@ PPRF1.f(xi, k);
+    x2 <@ PPRF1.f(xi, pk);
     return x1 = x2;
   }
 }.
@@ -69,24 +69,216 @@ rnd. skip. move => &hr xi_noteq_xp k _.
   smt().
 qed.
 
-    (* TODO: pprf indistinguishability *)
+(* Security Proofs Ideal/Real Setup *)
+
+  (* Security Notions *)
+module type PPRF = {
+  proc init(): unit
+  proc f(_ : D): R option
+  proc punc(_: D): unit
+}.
 
 
-clone import PRF as PRFa
-with type D <- D,
-type R <- R.
-   
-    (*
-module IND_PRF = PRFa.IND.
-module PRFi = PRF_RF.RF.
-(* Adv^PRG_PRGc(D) is defined as
-     Pr[IND_PRG(PRGc,D).main() @ &m: res]
-  - Pr[IND_PRG(PRGi,D).main() @ &m: res] *)
+module PPRF_Real: PPRF = {
+  var pk : PK
+
+  (* Gets a key from distribution dK and create pK with no punture point *)
+  proc init() : unit = {
+    var k;
+    var pk : PK;
+    k <$ dK;
+    pk <- {| key = k; x = None; |};
+  }
+
+  (* Puncture pK at point x if it is not already punctured, otherwise do nothing *)
+  proc punc(x: D): unit = {
+    if (pk.`x = None) {
+      pk <- {| key = pk.`key; x = Some x |};
+    }
+    
+  }
+
+  (* If pk is not puntured at x, return the value of PRF at x *)
+  proc f(x: D): R option  = {
+    var r : R option;
+    r <- if pk.`x = Some x then None else Some (F pk.`key x);
+    return r;
+  }
+}.
+
+section Correctness.
+
+lemma pprf_correctness_1 &m1 &m2 k xp xi o:
+    xp <> xi
+    /\ PPRF_Real.pk.`key{m1} = k
+    /\ PPRF_Real.pk.`key{m2} = k
+    /\ PPRF_Real.pk.`x{m1} = None
+    /\ PPRF_Real.pk.`x{m2} = Some xp
+    =>
+     Pr[PPRF_Real.f(xi) @ &m1 : res = o] = 
+     Pr[PPRF_Real.f(xi) @ &m2 : res = o].
+    proof.
+    move => [xp_xi_neq [m1k [mk2 [m1none mk2xp]]]].
+    byequiv => //.
+    proc; inline; wp; skip.
+    move => &1 &2.
+    smt.
+  qed.
+  
+lemma pprf_correctness_2 &m1 &m2 k xp xi o:
+    xp <> xi
+    /\ PPRF_Real.pk.`key{m1} = k
+    /\ PPRF_Real.pk.`key{m2} = k
+    /\ PPRF_Real.pk.`x{m1} = None
+    /\ PPRF_Real.pk.`x{m2} = Some xp
+    =>
+    equiv [PPRF_Real.f ~ PPRF_Real.f : true ==> ={res}.
+    proof.
+    move => [xp_xi_neq [m1k [mk2 [m1none mk2xp]]]].
+    byequiv => //.
+    proc; inline; wp; skip.
+    move => &1 &2.
+    move => [x2xieq [pk2 [x1xieq pk1]]].
+    admit.
+  qed.
+
+      (*
+
+          byequiv => //.
+      proc; inline; wp; skip;
+    move => &1 &2 h1. split.
+    move => h2 h3;
+      have same : x{1} = x{2} by smt();
+      have xi_xp : x{1} = xi by smt();
+      have nxp : PPRF_Real.pk{2}.`Top.x <> Some x{2} by smt.
+      have eqif1 : (if PPRF_Real.pk{2}.`Top.x = Some x{2} then None
+      else Some (F PPRF_Real.pk{2}.`key x{2})) = Some (F PPRF_Real.pk{2}.`key x{2}) by smt().
+      rewrite eqif1.
+      have pk1 : PPRF_Real.pk{1} = PPRF_Real.pk{m1} by smt.
+      have h2s :  PPRF_Real.pk{1}.`Top.x = None /\ PPRF_Real.pk{1}.`key = k => Some (F PPRF_Real.pk{1}.`key x{1}) =
+      o by smt().
+      *)
+
+  
+end section Correctness.
+ 
+require import FMap.
+op dR: { D -> R distr | forall x, is_lossless (dR x) /\ forall x, is_full (dR x)} as dR_ll.
+
+module PPRF_Ideal : PPRF = {
+  var m : (D,R) fmap
+  var punc_x : D option
+  var coll : bool
+
+  proc init(): unit = {
+    m  <- empty;
+    punc_x <- None;
+    coll <- false;
+  }
+
+  proc punc(x:D): unit = {
+    if (punc_x = None) {
+      punc_x <- Some x;
+    }
+  }
+
+  proc f(x:D): R option = {
+    var r;
+    if (x \notin m) {
+      r <$ dR x;
+      coll   <- coll \/ rng m r;
+      m.[x]  <- r;
+    }
+    return if punc_x = Some x then None else Some (oget m.[x]);
+  }
+
+}.
+
+module type PPRF_Oracles = {
+  proc f(_: D): R option
+}.
+
+module type Distinguisher (P: PPRF_Oracles) = {
+  proc distinguish(): bool
+}.
+
+    (* We limit our distiniguisher to have q calls *)
+    (* This is to express a computationally bounded adversary through a computationally bounded oracle *)
+
+op q : { int | 0 <= q } as ge0_q.
+
+module DBounder (D : Distinguisher) (F : PPRF_Oracles) = {
+  module FBounder = {
+    var c:int
+
+    proc f(x:D): R option = {
+      var r <- witness;
+      if (c < q) {
+        r <@ F.f(x);
+        c <- c + 1;
+      }
+      return r;
+    }
+  }
+
+  proc distinguish(): bool = {
+    var b;
+    FBounder.c <- 0;
+    b <@ D(FBounder).distinguish();
+    return b;
+  }
+}.
 
 
-*)
-    (* TODO: pprf unpredictability *)
+section BoundedPPRF.
 
+  (* 3 STEPS *)
+  (* Concretely bound the real PRF to a bounding based on number of calls *)
+  (* Prove PRF_Real ~ PRF_Ideal *)
+
+declare module D <: Distinguisher {-PPRF_Real, -DBounder}.
+
+(* Sometimes reductions can be lossy *) 
+declare axiom D_ll (O <: PPRF_Oracles {-D}): islossless O.f => islossless D(O).distinguish.
+
+module Exp_IND (P: PPRF) (D: Distinguisher) = {
+  proc main(): bool = {
+    var b;
+    P.init();
+    b <@ D(P).distinguish();
+    return b;
+  }
+}.
+
+op uD: { D distr | is_uniform uD /\ is_lossless uD /\ is_full uD } as uD_uf_fu.
+
+lemma PPRF_Collision_Strong &m:
+    Pr[Exp_IND(PPRF_Ideal, DBounder(D)).main() @ &m: PPRF_Ideal.coll]
+      <= (q^2 - q)%r / 2%r * mu uD (pred1 witness). (* (q^2 - q) / 2 * (1/|D|) *) (* q^2 - q / 2|D| *)
+proof.
+  admit. 
+qed.
+
+lemma PPRF_Collision_Weak &m:
+    Pr[Exp_IND(PPRF_Ideal, DBounder(D)).main() @ &m: PPRF_Ideal.coll]
+      <= (q^2)%r * mu uD (pred1 witness). (* (q^2) / (1/|D|) *)
+proof.
+  admit. 
+qed.
+
+
+end section BoundedPPRF.
+
+section RealIdealIND.
+
+declare module D <: Distinguisher {-PPRF_Real, -PPRF_Ideal}.
+
+lemma RealIdeal &m : Pr[Exp_IND(PPRF_Real,D).main() @ &m: res] = Pr[Exp_IND(PPRF_Ideal,D).main() @ &m: res].
+proof.
+  admit.
+qed.
+
+end section RealIdealIND.
 
 
 
@@ -98,9 +290,9 @@ module Experiement3 = {
   proc f(x: D): R option = {
     var r;
     var pk;
-    pk <@ PuncturablePsuedoRF.init();
-    pk <@ PuncturablePsuedoRF.puncture(x, pk);
-    r <@ PuncturablePsuedoRF.f(x, pk);
+    pk <@ PPRF1.init();
+    pk <@ PPRF1.puncture(x, pk);
+    r <@ PPRF1.f(x, pk);
     return r;
   }
 }. 
@@ -109,8 +301,8 @@ module Experiement4 = {
   proc f(x: D): R option = {
     var r;
     var pk;
-    pk <@ PuncturablePsuedoRF.init();
-    r <@ PuncturablePsuedoRF.f(x, pk);
+    pk <@ PPRF1.init();
+    r <@ PPRF1.f(x, pk);
     return r;
   }
 }. 
